Remove unused definitions + add various lemmas
* Removed theorems and definitions based on old versions of the transformation
  or otherwise unused things.
* Worked some on evaluate_optimized theorem.
* Removed impure case from op_rewrite. `f x + f y` type expressions are
  not supported.
* Added lemmas about op_identity.
* Repaired some proofs.

compiler/backend/bvi_tailrecScript.sml
@@ -66,7 +66,6 @@ val id_from_op_def = Define `
   (id_from_op _             = bvi$Var 65534) (* dummy *)
   `;
 
-(* Get the sub-expressions from a binary operation *)
 val op_binargs_def = Define `
   op_binargs (bvi$Op _ [e1; e2]) = SOME (e1, e2) ∧
   op_binargs _                   = NONE
@@ -87,124 +86,11 @@ val is_pure_def = tDefine "is_pure" `
   (WF_REL_TAC `measure exp_size` \\ rw []
   \\ imp_res_tac MEM_exp_size_imp \\ fs []);
 
-(* Purity modulo call to `name` *)
-val is_pure_mod_rec_def = Define `
-  (is_pure_mod_rec name (Call _ (SOME n) _ _) ⇔ n = name) ∧
-  (is_pure_mod_rec name exp                   ⇔ is_pure exp)
-  `;
-
-val op_binargs_exp_size = Q.store_thm ("op_binargs_exp_size",
-  `∀xs x1 x2. op_binargs xs = SOME (x1, x2) ⇒
-    (exp_size x1 < exp_size xs ∧ exp_size x2 < exp_size xs)`,
-  Induct \\ fs [op_binargs_def]
-  \\ Cases_on `l` \\ fs [op_binargs_def]
-  \\ Cases_on `t` \\ fs [op_binargs_def]
-  \\ Cases_on `t'` \\ fs [op_binargs_def]
-  \\ rw [bviTheory.exp_size_def]);
-
-(* Decompose a series of nested operator applications (provided the operators
-   are the same) into a list of operands by in-order traversal. *)
-val decomp_def = tDefine "decomp" `
-  decomp op exp =
-    if ¬op_eq op exp then
-      [exp]
-    else
-      case op_binargs exp of
-      | SOME (e1, e2) => decomp op e1 ++ decomp op e2
-      | NONE          => [exp]`
-  (WF_REL_TAC `measure (exp_size o SND)` \\ rw []
-  \\ imp_res_tac op_binargs_exp_size \\ fs []);
-
-(* Check if the call is recursive to `name` *)
 val is_rec_def = Define `
   (is_rec name (bvi$Call _ d _ _) ⇔ d = SOME name) ∧
   (is_rec _    _                  ⇔ F)
   `;
 
-(* Check if the expression is tail recursive wrt calls to `n` *)
-val is_tailrec_def = Define `
-  (is_tailrec n (If _ x2 x3)          ⇔ is_tailrec n x2 ∨ is_tailrec n x3) ∧
-  (is_tailrec n (Let _ x1)            ⇔ is_tailrec n x1) ∧
-  (is_tailrec n (Tick x1)             ⇔ is_tailrec n x1) ∧
-  (is_tailrec n (Call _ (SOME m) _ _) ⇔ n = m) ∧
-  (is_tailrec n _                     ⇔ F)`;
-
-(* Ensure that all expressions /after/ the first recursive call in an in-order
-   traversal are pure. *)
-val all_pure_mod_rec_def = Define `
-  (all_pure_mod_rec name has_rec []      ⇔ T) ∧
-  (all_pure_mod_rec name has_rec (x::xs) ⇔
-    if is_rec name x then
-      all_pure_mod_rec name T xs
-    else
-      (has_rec ⇒ is_pure_mod_rec name x) ∧
-      all_pure_mod_rec name has_rec xs)
-  `;
-
-(* Check call arguments for recursive calls. Returns the accepted
-   decomposition if successful.
-
-   TODO: This is wrong
-*)
-val arg_check_app_def = Define `
-  arg_check_app op name op1 =
-    let ds = decomp op op1 in
-    let len = LENGTH ds in
-      if len ≤ 1 then
-        NONE
-      else
-        if is_rec name (HD ds) ∧ all_pure_mod_rec name F ds then
-          SOME ds
-        else
-          NONE
-  `;
-
-(* Given that addition and multiplication are commutative operations, the place
-   in which the recursive call appears is not important, as long as it appears
-   at all, and that all expressions prior to this call in the in-order are pure,
-   so that side-effects are not evaluated out of order. *)
-val arg_check_int_def = Define `
-  arg_check_int op name op1 =
-    let ds = decomp op op1 in
-    let len = LENGTH ds in
-      if len ≤ 1 then
-        NONE
-      else
-        if EXISTS (is_rec name) ds ∧ all_pure_mod_rec name F ds then
-          SOME ds
-        else
-          NONE
-  `;
-
-(* Check tail positions for operators containing tail calls. The first
-   operator found with optimizable sub-expressions is returned. *)
-
-(*
-val tail_check_def = Define `
-  (tail_check name (Var _)        = NONE) ∧
-  (tail_check name (Let _ x1)     = tail_check name x1) ∧
-  (tail_check name (Tick x1)      = tail_check name x1) ∧
-  (tail_check name (Raise x1)     = NONE) ∧
-  (tail_check name (If _ x2 x3)   =
-    case tail_check name x2 of
-    | SOME op => SOME op
-    | _       => tail_check name x3) ∧
-  (tail_check name (Call _ _ _ _) = NONE) ∧
-  (tail_check name (Op op xs)     =
-    if op = Add ∨ op = Mult then
-      let op1 = from_op op in
-        (case arg_check_int op1 name (Op op xs) of
-        | SOME _ => SOME op1
-        | _ => NONE)
-    else NONE)`;
-*)
-
-(* Ensure that return values in sub-expressions are literals, arithmetic, or
-   recursive calls to the function itself.
-
-   TODO: All tail positions will need to be modified with some no-op arithmetic
-   before this point, e.g. x |-> x + 0.
-*)
 val ok_tail_type_def = Define `
   (ok_tail_type name (Op op _)             ⇔ is_arithmetic op) ∧
   (ok_tail_type name (Call _ (SOME n) _ _) ⇔ n = name) ∧
@@ -214,103 +100,6 @@ val ok_tail_type_def = Define `
     ok_tail_type name x2 ∧ ok_tail_type name x3) ∧
   (ok_tail_type name _                     ⇔ F)
   `;
-
-(* Pick out the first recursive call to `name` and return it together with the
-   list up to and following that point so that
-
-     comp name qs xs = (front, call, back) ⇒ front ++ [call] ++ back = xs
-
-  TODO could return the parameters to the call instead *)
-val comp_def = Define `
-  (comp name qs []      = (REVERSE qs, Call 23583 NONE [] NONE, [])) ∧
-  (comp name qs (x::xs) =
-    if is_rec name x then (REVERSE qs, x, xs) else comp name (x::qs) xs)
-  `;
-
-(* TODO this could take parameters (t,d,as,h) *)
-val setup_call_def = Define `
-  (setup_call n acc op exp (SOME (t,d,as,hdl)) =
-    Call t (SOME n) ((apply_op op (Var acc) exp)::as) hdl) ∧
-  (setup_call n acc op exp NONE = Call 35505 NONE [] NONE) (* dummy *)
-  `;
-
-(* We REVERSE xs since we want the /last/ recursive call *)
-val mk_tailcall_int_def = Define `
-  mk_tailcall_int n op name acc xs =
-    let (front, call, back) = comp name [] (REVERSE xs) in
-    let ys = (REVERSE back) ++ (REVERSE front) in
-      setup_call n acc op (FOLDR (apply_op op) (LAST ys) (FRONT ys)) 
-                          (args_from call)
-  `;
-
-(* Attempt to rewrite tail positions matching `op` with tail calls. All other
-   tail positions are rewritten by applying the accumulator from the right. *)
-
-(*
-val tail_rewrite_def = Define `
-  (tail_rewrite n op name acc (Let xs x1) =
-    Let xs (tail_rewrite n op name (acc + LENGTH xs) x1)) ∧
-  (tail_rewrite n op name acc (Tick x1) =
-    Tick (tail_rewrite n op name acc x1)) ∧
-  (tail_rewrite n op name acc (Raise x1) = Raise x1) ∧
-  (tail_rewrite n op name acc (If x1 x2 x3) =
-    let y2 = tail_rewrite n op name acc x2 in
-    let y3 = tail_rewrite n op name acc x3 in
-      If x1 y2 y3) ∧
-  (tail_rewrite n op name acc exp =
-    case arg_check_int op name exp of
-    | NONE    => apply_op op exp (Var acc)
-    | SOME ds => mk_tailcall_int n op name acc ds)
-  `;
-
-*)
-
-(* -------------------------------------------------------------------------- *)
-
-
-(* Recursively rewrite. Try to achieve things like:
-
-     1 + length xs |-> length xs + 1    since is_pure 1
-
-   For instance, if we receive (op_rewrite x1, op_rewrite x2) = 
-
-     (1) (e1, f1 xs + y) ∧ is_pure e1     |-> (T, f1 xs + (y + e1)) 
-     (2) (f1 xs + y, e2) ∧ is_pure e2     |-> (T, f1 xs + (y + e2))
-     (3) (f1 xs + y, f2 xs + z)           |-> (T, f2 xs + (y + (f1 xs + z)))
-     (4) otherwise                        |-> (F, apply_op x1 x2)
-
-   In (3), f1, f2 are both recursive calls to "our" function. to preserve order
-   of potential side-effects, use the rightmost one outermost (evaluate last).
-
-   Finally, if there was a rewrite, i.e. (T, exp) returns, then we know that
-   
-     ∃ticks args hdl exp2. 
-       exp = apply_op op (Call ticks (SOME name) args hdl) exp2
-
-   We then rewrite this to 
-
-     Call ticks (SOME n) (apply_op op (Var acc) exp2 :: args) hdl.
-
-   Otherwise if we get (F, exp) we just replace it with
-
-     apply_op op exp (Var acc)
-
-   Hopefully we can derive some lemmas because correctness locally here seems to
-   imply correcntess globally when composing the expressions.
-
-   Because of associativity and commutativity, the original exp and the result 
-   in (F/T, exp) should be equivalent. Moreover, each step in the recursion
-   should produce an equivalent result. If we have some associativity lemma
-   for apply op we should be able to do induction on op_rewrite and say that
-
-      evaluate ([exp], env, s) = (r, t) ∧
-      r ≠ Rerr (Rabort Rtype_error) ⇒ 
-        case op_rewrite op exp of
-        | (F, exp2) => exp = exp2 
-        | (T, exp2) => evaluate ([exp2], env, s) = (r, t)
-
-   _Maybe_.
-*)
 
 val binop_has_rec_def = Define `
   binop_has_rec name op exp ⇔
@@ -354,7 +143,8 @@ val op_rewrite_def = tDefine "op_rewrite" `
         let (r2, y2) = op_rewrite op name x2 in
           case (binop_has_rec name op y1, binop_has_rec name op y2) of
           | (F, F) => (F, exp)
-          | (T, T) => (T, ac_swap op y1 y2)
+          (*| (T, T) => (T, ac_swap op y1 y2)*)
+          | (T, T) => (F, exp)
           | (T, F) => if is_pure y2 then (T, ac_swap op y2 y1) else (F, exp)
           | (F, T) => if is_pure y1 then (T, ac_swap op y1 y2) else (F, exp)
   `
@@ -363,10 +153,6 @@ val op_rewrite_def = tDefine "op_rewrite" `
   \\ drule exp_size_op_binargs
   \\ fs []);
 
-(* Use the rewrite function as the new ``tail_check``. If it succeeds it should
-   be fine?
-*)
-   
 val tail_check_def = Define `
   (tail_check name (Var _)        = NONE) ∧
   (tail_check name (Let _ x1)     = tail_check name x1) ∧
@@ -402,7 +188,6 @@ val mk_tailcall_def = Define `
           push_call n op acc exp3 (args_from call))
   `;
 
-(* New tail_rewrite function *)
 val tail_rewrite_def = Define `
   (tail_rewrite n op name acc (Let xs x1) =
     Let xs (tail_rewrite n op name (acc + LENGTH xs) x1)) ∧
@@ -416,10 +201,6 @@ val tail_rewrite_def = Define `
   (tail_rewrite n op name acc exp = mk_tailcall n op name acc exp)
   `;
 
-(* -------------------------------------------------------------------------- *)
-
-(* If the type of the tail positions is determined to be fine we check if there
-   is some tail position that can be optimized. *)
 val optimize_check_def = Define `
   optimize_check name exp =
     if ¬ok_tail_type name exp then
@@ -428,26 +209,16 @@ val optimize_check_def = Define `
       tail_check name exp
   `;
 
-(* The accumulator is the first variable in the environment. However,
-   all other variables in the expression need to be shifted up one step.
-
-   If we wrap the expression in a Let expression we won't have to traverse the
-   expression and selectively shift some variables up; pretending that the
-   accumulator is at the very end of the environment when optimizing will
-   suffice. In short, we prepend the environment with its tail, and the
-   accumulator ends up in the right place. *)
 val let_wrap_def = Define `
   let_wrap num_args exp =
     Let (GENLIST (λi. Var (i + 1)) num_args) exp
   `;
 
-(* Create auxilliary definition (use the "old" name). *)
 val mk_aux_call_def = Define `
   mk_aux_call name num_args id =
     Call 0 (SOME name) (id :: GENLIST (λi. Var (i + 0)) num_args) NONE
   `;
 
-(* Perform the full rewrite and generate an auxilliary function. *)
 val optimize_single_def = Define `
   optimize_single n name num_args exp =
     case optimize_check name exp of
@@ -456,21 +227,6 @@ val optimize_single_def = Define `
         let opt = let_wrap num_args (tail_rewrite n op name num_args exp) in
         let aux = mk_aux_call n num_args (id_from_op op) in
           SOME (aux, opt)
-  `;
-
-(* Applies the tail-recursion optimization on all entries in the code table.
-   Requires the first free name in the code table following the renaming in
-   BVL-to-BVI. *)
-val optimize_all_def = Define `
-  (optimize_all n code []                    acc = REVERSE acc) ∧
-  (optimize_all n code ((nm, args, exp)::xs) acc =
-    case optimize_single n nm args exp of
-    | NONE => optimize_all n code xs ((nm, args, exp)::acc)
-    | SOME (exp_aux, exp_opt) =>
-        let code1 = insert nm (args, exp_aux) code in
-        let code2 = insert n (args + 1, exp_opt) code1 in
-          optimize_all (n + 2) code2 xs
-            ((nm, args, exp_aux)::(n, args + 1, exp_opt)::acc))
   `;
 
 val optimize_prog_def = Define `
